\documentclass{article}
\usepackage{amsmath}
\begin{document}
\begin{equation}
\frac{\partial \mathcal{L}(w, w_0, \xi, \lambda, \mu)}{\partial w} = 0 \quad \Longrightarrow \quad w = \sum_{i=1}^N \lambda_i y_i x_i
\end{equation}

\begin{equation}
\frac{\partial \mathcal{L}(w, w_0, \xi, \lambda, \mu)}{\partial w_0} = 0 \quad \Longrightarrow \quad \sum_{i=1}^N \lambda_i y_i = 0
\end{equation}

\begin{equation}
\frac{\partial \mathcal{L}(w, w_0, \xi, \lambda, \mu)}{\partial \xi_i} = 0 \quad \Longrightarrow \quad C - \mu_i - \lambda_i = 0
\end{equation}

Putting (4), (5) and (6) into $\mathcal{L}(w, w_0, \xi, \lambda, \mu)$, we have

\begin{align}
\mathcal{L}(\lambda, \xi) &= \frac{1}{2}||w||^2 + C\sum_{i=1}^N \xi_i - \sum_{i=1}^N \mu_i \xi_i - \sum_{i=1}^N \lambda_i(y_i(w^T x_i + w_0) - 1 + \xi_i) \\
&= \frac{1}{2}\sum_{i=1}^N \sum_{j=1}^N \lambda_i \lambda_j y_i y_j x_i^T x_j + C\sum_{i=1}^N \xi_i - \sum_{i=1}^N \mu_i \xi_i - \sum_{i=1}^N \lambda_i y_i w^T x_i - \sum_{i=1}^N \lambda_i y_i w_0 + \sum_{i=1}^N \lambda_i - \sum_{i=1}^N \lambda_i \xi_i \\
&= \frac{1}{2}\sum_{i=1}^N \sum_{j=1}^N \lambda_i \lambda_j y_i y_j x_i^T x_j + C\sum_{i=1}^N \xi_i - \sum_{i=1}^N \mu_i \xi_i - \sum_{i=1}^N \lambda_i y_i \left( \sum_{j=1}^N \lambda_j y_j x_j^T \right) x_i - \sum_{i=1}^N \lambda_i y_i w_0 + \sum_{i=1}^N \lambda_i - \sum_{i=1}^N \lambda_i \xi_i \\
&= \sum_{i=1}^N \lambda_i - \frac{1}{2}\sum_{i=1}^N \sum_{j=1}^N \lambda_i \lambda_j y_i y_j x_i^T x_j.
\end{align}
\end{document}